Main.lean
@@ -8,69 +8,92 @@ import ContraProof.Verification
 -- ==========================================
 
 -- The Baby Yoda: starting state is improper w/neighbor swing
-def babyYoda : Dance := [
-  circleLeft 3 8,
-  inPlace "Partners do si do once" 8,
-  inPlace "Partners balance" 4,
-  sideSwing "Partners swing" 12,
-  robinsChain 8,
-  leftStar 4 8,
-  progress "Onto new neighbors" 0, -- Pushes dancers into the adjacent set
-  inPlace "New Neighbor Balance" 4,
-  sideSwing "Neighbors swing" 12
-]
+def babyYoda : Dance := {
+  name := "The Baby Yoda",
+  beats := 64,
+  startingFormation := initialImproperWithNeighborSideSwing,
+  figures := [
+    circleLeft 3 8,
+    inPlace "Partners do si do once" 8,
+    inPlace "Partners balance" 4,
+    sideSwing "Partners swing" 12,
+    robinsChain 8,
+    leftStar 4 8,
+    progress "Onto new neighbors" 0, -- Pushes dancers into the adjacent set
+    inPlace "New Neighbor Balance" 4,
+    sideSwing "Neighbors swing" 12
+  ]
+}
 
 -- The Baby Rose, should pass tests
-def babyRose : Dance := [
-  inPlace "New Neighbor Balance" 4,
-  sideSwing "Neighbors swing" 12,
-  circleLeft 3 8,
-  inPlace "Partners do si do once" 8,
-  inPlace "Partners balance" 4,
-  sideSwing "Partners swing" 12,
-  robinsChain 8,
-  leftStar 4 8,
-  -- Pushes dancers into the adjacent set & checks direction of travel
-  progress "Onto new neighbors" 0
-]
+def babyRose : Dance := {
+  name := "The Baby Rose",
+  beats := 64,
+  startingFormation := initialImproper,
+  figures := [
+    inPlace "New Neighbor Balance" 4,
+    sideSwing "Neighbors swing" 12,
+    circleLeft 3 8,
+    inPlace "Partners do si do once" 8,
+    inPlace "Partners balance" 4,
+    sideSwing "Partners swing" 12,
+    robinsChain 8,
+    leftStar 4 8,
+    -- Pushes dancers into the adjacent set & checks direction of travel
+    progress "Onto new neighbors" 0
+  ]
+}
 
 -- Easy Peasy by Diane Silver, should pass tests
-def easyPeasy : Dance := [
-  inPlace "New Neighbor Balance" 4,
-  sideSwing "Neighbors swing" 12,
-  inPlace "Long lines forward back" 8,
-  allemandeLarks 6 8,
-  inPlace "Partners balance" 4,
-  sideSwing "Partners swing" 12,
-  circleLeft 3 8,
-  inPlace "Balance the ring" 4,
-  caliTwirl "Partners California Twirl" 4,
-  -- Pushes dancers into the adjacent set & checks direction of travel
-  progress "Onto new neighbors" 0
-]
+def easyPeasy : Dance := {
+  name := "Easy Peasy",
+  beats := 64,
+  startingFormation := initialImproper,
+  figures := [
+    inPlace "New Neighbor Balance" 4,
+    sideSwing "Neighbors swing" 12,
+    inPlace "Long lines forward back" 8,
+    allemandeLarks 6 8,
+    inPlace "Partners balance" 4,
+    sideSwing "Partners swing" 12,
+    circleLeft 3 8,
+    inPlace "Balance the ring" 4,
+    caliTwirl "Partners California Twirl" 4,
+    -- Pushes dancers into the adjacent set & checks direction of travel
+    progress "Onto new neighbors" 0
+  ]
+}
 
 -- ==========================================
 -- VERIFICATION TESTS
 -- ==========================================
 
--- Check if the total beat count equals 64
-#eval checkPhrasing babyYoda
-#eval checkPhrasing babyRose
-#eval checkPhrasing easyPeasy
+-- Test Baby Rose
+#eval checkBeats babyRose
+#eval checkProgressive babyRose
+theorem babyRose_phrasing : ValidBeats babyRose := rfl
+theorem babyRose_progression : IsProgressive babyRose := rfl
 
--- Check if the topology successfully progresses the couples
-#eval checkProgressive babyYoda initialImproperWithNeighborSideSwing
-#eval checkProgressive babyRose initialImproper
-#eval checkProgressive easyPeasy initialImproper
+-- Test Baby Yoda
+#eval checkBeats babyYoda
+#eval checkProgressive babyYoda
+theorem babyYoda_phrasing : ValidBeats babyYoda := rfl
+theorem babyYoda_progression : IsProgressive babyYoda := rfl
 
+
+-- Test Easy Peasy
+#eval checkBeats easyPeasy
+#eval checkProgressive easyPeasy
+theorem easyPeasy_phrasing : ValidBeats easyPeasy := rfl
+theorem easyPeasy_progression : IsProgressive easyPeasy := rfl
 
 
 def main : IO Unit := do
   IO.println "Evaluating The Baby Yoda Phrasing (Expect true):"
-  IO.println (checkPhrasing babyYoda)
-  IO.println "\nEvaluating The Baby Yoda Progression (Expect false):"
-  IO.println (checkProgressive babyYoda initialImproper)
+  IO.println (checkBeats babyYoda)
+  IO.println "\nEvaluating The Baby Yoda Progression (Expect true):"
+  IO.println (checkProgressive babyYoda)
   IO.println "Evaluating The Baby Rose Phrasing (Expect true):"
-  IO.println (checkPhrasing babyRose)
+  IO.println (checkBeats babyRose)
   IO.println "\nEvaluating The Baby Rose Progression (Expect true):"
-  IO.println (checkProgressive babyRose initialImproper)
+  IO.println (checkProgressive babyRose)
